src/Language/PlutusIR/Semantics/Dynamic/AnnotationSubstitution/PreservesValue.v
@@ -1,0 +1,36 @@
+Require Import PlutusCert.Language.PlutusIR.
+Import NamedTerm.
+Require Import PlutusCert.Language.PlutusIR.Semantics.Static.
+
+Require Import PlutusCert.Language.PlutusIR.Semantics.Dynamic.Values.
+Require Import PlutusCert.Language.PlutusIR.Semantics.Dynamic.AnnotationSubstitution.
+
+
+
+Theorem substituteA_preserves_value : forall v v' a T,
+    value v ->
+    substituteA a T v v' ->
+    value v'.
+Proof.
+  intros.
+  inversion H; subst; try solve [inversion H0; subst; auto]. 
+Admitted.
+
+Theorem msubstA_preserves_value : forall envA v v',
+    value v ->
+    msubstA envA v v' ->
+    value v'.
+Proof.
+  induction envA.
+  - intros.
+    inversion H0.
+    subst.
+    assumption.
+  - intros.
+    inversion H0.
+    subst.
+    eapply IHenvA.
+    + eapply substituteA_preserves_value; eauto.
+    + eauto.
+Qed. 
+
